going over some examples of linked list with Ruxandra

state/LinkedListIFC.fst
@@ -11,88 +11,106 @@ open TargetLangIFC
 
 module FSet = FStar.FiniteSet.Base
 
-let head_tot (#a: Type0) (l: linkedList a{l =!= Nil}) (h: lheap) {| c: witnessable a |} : a =
-  let Cons(x, xsref) = l in
- x
-
-let tail_tot (#a: Type0) (l: linkedList a) (h: lheap) {| c: witnessable a |} : linkedList a = 
-    match l with
-      | Nil -> Nil
-      | Cons (x, xsref) -> 
-        assume (satisfy l h contains_pred);
-        sel_tot h xsref
-
-let rec ll_eq (#a: Type0) (fuel: nat) (l1: linkedList a) (l2: linkedList a) (h: lheap) : Type0 =
-  if fuel = 0 then True
+let rec ll_eq (#a: Type0) (step: nat) (l1: linkedList a) (l2: linkedList a) (h: lheap) : Type0 =
+  if step = 0 then True
   else
     match (l1, l2) with
     | (Nil, Nil) -> true
     | Nil, _ -> false
     | _, Nil -> false
-    | (Cons (x, xsref), Cons (y, ysref)) ->
+    | Cons x xsref, Cons y ysref ->
       let xs = sel h xsref in
       let ys = sel h ysref in  
-      x == y /\ ll_eq (fuel - 1) xs ys h
+      x == y /\ ll_eq (step - 1) xs ys h
+
+let head_tot (#a: Type0) (l: linkedList a{l =!= Nil}) (h: lheap) : a =
+  let Cons x xsref = l in
+  x
 
 let head (#a: Type0) (l:linkedList a) {| c:witnessable a |} : IST (option a)
   (requires fun h -> l =!= Nil)
-  (ensures fun h0 head h1 -> modifies_none h0 h1 /\ head == Some (head_tot l h1)) =
+  (ensures fun h0 head h1 -> h0 == h1 /\ head == Some (head_tot l h1)) =
       match l with
       | Nil -> None
-      | Cons (x, xsref) -> Some x
+      | Cons x xsref -> Some x
 
-let tail (a: Type0) (l: linkedList a) {| c:witnessable a |} : IST (linkedList a)
+let tail_tot (#a: Type0) (l: linkedList a) (h: lheap) : 
+  Pure (linkedList a)
+    (requires (Cons? l ==> h `contains` (Cons?.next l)))
+    (ensures (fun _ -> True)) = 
+  match l with
+  | Nil -> Nil
+  | Cons x xsref -> sel_tot h xsref
+
+let tail (a: Type0) (l: linkedList a) {| c:witnessable a |} : 
+  IST (linkedList a)
     (requires fun h -> satisfy l h contains_pred)
-    // try to use tail_tot in the postcondition
-    (ensures fun h0 xs h1 -> True) = 
-      match l with
-      | Nil -> Nil
-      | Cons (x, xsref) -> !xsref
+    (ensures (fun h0 xs h1 -> h0 == h1 /\ xs == tail_tot l h0)) = 
+  match l with
+  | Nil -> Nil
+  | Cons x xsref -> 
+    let h = get () in
+    lemma_sel_equals_sel_tot_for_contained_refs h xsref;
+    !xsref
 
-(* TODO: can we do this for l: linkedlist a? *)
-  // let rec last_elem (l: linkedList nat) {| c:witnessable nat |} : IST (option nat)
-  // (requires (fun h -> satisfy l h contains_pred))
-  // (ensures fun _ _ _ -> True) = 
-  //   let h0 = get() in
-  //   match l with 
-  //   | Nil -> None
-  //   | Cons (x, xsref) ->
-  //     let xs = !xsref in
-  //     match xs with
-  //     | Nil -> Some x
-  //     | Cons _ -> 
-  //       eliminate_inv_contains h0 (TLList TNat) xsref;
-  //       last_elem xs #c
+// let rec ll_has_length (#a: Type0) (h: lheap) (l: linkedList a) (len:nat) : Type0 =
+//   l == Nil \/ (ll_has_length h (Cons?.next l) (len - 1))
 
-// let rec last_ref (#a: Type0) (l:linkedList a{l =!= Nil}) (h: lheap) : GTot (ref (linkedList a)) =
-//   let Cons (x, xsref) = l in
+// let rec last_ref (#a: Type0) (l:linkedList a{l =!= Nil}) (h: lheap) : option (linkedList a) =
+//   let Cons x xsref = l in
 //   assume (h `contains` xsref);
-//    let xs = sel h xsref in
-//    match xs with
-//     | Nil -> xsref
-//     | Cons _ -> last_ref #a xs h
+//   let xs = sel_tot h xsref in
+//   match xs with
+//   | Nil -> Some l
+//   | Cons _ _ -> last_ref #a xs h
+
+let rec last_elem (t:typ) (l: elab_typ (TLList t)) : 
+  IST (option (elab_typ t))
+    (requires (fun h -> (elab_typ_tgt (TLList t)).satisfy l h contains_pred))
+    (ensures fun h0 _ h1 -> h0 == h1) = 
+  let h0 = get () in
+  let l : linkedList (elab_typ t) = l in
+  match l with 
+  | Nil -> None
+  | Cons x xsref ->
+    let xs = !xsref in
+    match xs with
+    | Nil -> Some x
+    | Cons _ _ -> 
+      eliminate_inv_contains h0 (TLList t) xsref;
+      last_elem t xs
 
 
-let insert_front (a: Type0) (l: linkedList a) (v: a) {| c:witnessable a |}: ST (linkedList a)
+let insert_front (#a: Type0) (l: linkedList a) (v: a) : 
+  ST (linkedList a)
     (requires (fun _ -> True))
-    (ensures fun _ _ _ -> True) = 
-    let r: ref (linkedList a) = alloc l in 
-    Cons (v, r)
+    (ensures fun h0 _ h1 -> True) = 
+  let r: ref (linkedList a) = alloc l in 
+  Cons v r
 
 // TODO: fix this
-// let rec append (a: Type0) (l: linkedList a) (v: a) {| c:target_lang a |}: IST (linkedList a)
-//     (requires (fun h -> shallowly_contained l h /\ shallowly_low l h))
-//     (ensures fun _ _ _ -> True) =
-//     let h0 = get() in
-//     match l with
-//     | Nil -> 
-//       let r = alloc Nil in 
-//       Cons (v, r)
-//     | Cons (v, r) -> 
-//       let tl = !r in
-//         eliminate forall (a:Type) (c:target_lang a) (r':ref a). shallowly_low r' h0 ==>
-//         c.shallowly_low (sel h0 r') h0 with (linkedList a) (solve) r;
-//         append a tl v #c
+let rec append (#t: typ) (l: elab_typ (TLList t)) (v: elab_typ t) :
+  ST (elab_typ (TLList t))
+    (requires (fun h -> 
+      (elab_typ_tgt (TLList t)).satisfy l h contains_pred /\ 
+      inv_contains_points_to_contains h))
+    (ensures fun _ _ _ -> True) =
+  let h0 = get () in
+  let l : linkedList (elab_typ t) = l in
+  match l with
+  | Nil -> 
+    let r = alloc Nil in 
+    Cons v r
+  | Cons v r -> 
+    let tl = !r in
+    match tl with
+    | Nil -> 
+      let newr = alloc Nil in 
+      write r (Cons v newr);
+      l
+    | Cons _ _ -> 
+      eliminate_inv_contains h0 (TLList t) r;
+      append tl v
 
 // let rec length_IST (a: Type0) (l: linkedList a) {| c:witnessable a |} : IST nat 
 //        (requires (fun h -> shallowly_contained_low l h))
@@ -127,39 +145,40 @@ let rec deep_high_ll (#a: Type0) (fuel: nat) (l: linkedList a) (h: lheap): Type0
   else
     match l with
     | Nil -> True
-    | Cons (x, xsref) -> 
+    | Cons x xsref -> 
       label_of xsref h == High /\ deep_high_ll (fuel - 1) (sel h xsref) h
 
 noeq type deep_high_ll_ind (#a: Type0) (h: lheap) : linkedList a -> Type0 =
 | DH_Nil: deep_high_ll_ind #a h Nil
 | DH_Cons: x:a -> xsref: ref(linkedList a){label_of xsref h == High} ->
     deep_high_ll_ind h (sel h xsref) ->
-    deep_high_ll_ind h (Cons (x, xsref))
+    deep_high_ll_ind h (Cons x xsref)
 
 noeq type ll_constant_ind (#a: Type0) (h1 h2: lheap) : linkedList a -> Type0 =
 | LLC_Nil : ll_constant_ind h1 h2 (Nil #a)
 | LLC_Cons_Cons_Cons : v:a ->
     xsref:ref (linkedList a){sel h1 xsref == sel h2 xsref} ->
     ll_constant_ind h1 h2 (sel h1 xsref) ->
-    ll_constant_ind h1 h2 (Cons (v,xsref))
+    ll_constant_ind h1 h2 (Cons v xsref)
 
 let rec ll_constant (#a: Type0) (fuel: nat) (l: linkedList a) (h1 h2: lheap) : Type0 =
   if fuel = 0 then False
   else
     match l with
     | Nil -> True
-    | Cons (_, xsref) -> begin
+    | Cons _ xsref -> begin
       let xs1 = sel h1 xsref in
       let xs2 = sel h2 xsref in
       match (xs1, xs2) with
       | (Nil, Nil) -> True
       | Nil, _ -> False
       | _, Nil -> False
-      | (Cons (x, xsref), Cons (y, ysref)) ->
+      | (Cons x xsref, Cons y ysref) ->
         x == y /\ xsref == ysref /\ ll_constant (fuel - 1) xs1 h1 h2
     end
 
 
+#push-options "--split_queries always"
 let rec footprint_acc
   (#a: Type)
   (l: linkedList a) 
@@ -169,7 +188,7 @@ let rec footprint_acc
   Tot (erased (FSet.set pos)) (decreases (FSet.cardinality (hdom `FSet.difference` acc))) =
   match l with 
   | Nil -> acc
-  | Cons (x, xsref) -> 
+  | Cons x xsref -> 
     if addr_of xsref `FSet.mem` acc then acc
     else begin
       assume (h `contains` xsref);
@@ -184,10 +203,12 @@ let rec footprint_acc
               FSet.cardinality (hdom `FSet.difference` acc));
       footprint_acc (sel h xsref) h hdom acc' 
     end
+#pop-options
 
 let footprint (#a: Type) (l: linkedList a) (h:lheap) =
   let hdom = get_hdom h in
-  assume (FSet.emptyset `FSet.subset` hdom);
+  FSet.all_finite_set_facts_lemma ();
+  assert (FSet.emptyset `FSet.subset` hdom);
   footprint_acc l h hdom FSet.emptyset
 
 let separated (#a: Type) (l1 l2: linkedList a) (h: lheap): Type0 = 
@@ -198,25 +219,67 @@ let separated (#a: Type) (l1 l2: linkedList a) (h: lheap): Type0 =
 let empty_ll: linkedList nat = Nil
 
 let ll1 () : ST (linkedList nat) (requires fun _ -> True) (ensures fun _ _ _ -> True) =
-     let r: ref(linkedList nat) = alloc Nil in 
-     Cons (13, r)
+  let r: ref (linkedList nat) = alloc Nil in 
+  Cons 13 r
 
 let ll2 () : ST (linkedList nat) (requires fun _ -> True) (ensures fun _ _ _ -> True) =
-     let x = alloc Nil in 
-     let y = alloc (Cons (31, x)) in
-     let z = alloc (Cons (23, y)) in
-     Cons(23, z)
+  let x = alloc Nil in 
+  let y = alloc (Cons 31 x) in
+  let z = alloc (Cons 23 y) in
+  Cons 23 z
 
 let cycle_length3 () : ST (linkedList nat) (requires fun _ -> True) (ensures fun _ _ _ -> True) =
     let x = alloc Nil in 
-    let y = alloc (Cons (7, x)) in
-    let z = alloc (Cons (5, y)) in 
+    let y = alloc (Cons 7 x) in
+    let z = alloc (Cons 5 y) in 
     // gst_witness (contains_pred x);
-    write x (Cons(2, z));
-    Cons (2, z)
+    write x (Cons 2 z);
+    Cons 2 z
 
 
 // TODO: clean up
+let rec deep_declassify (l: linkedList int) : IST unit 
+  (requires fun h -> 
+    satisfy l h contains_pred)
+  (ensures fun h0 x h1 ->
+    modifies Set.empty h0 h1 /\
+    (* TODO: modifies_classification (footprint l) h0 h1 *)
+    satisfy l h1 is_low_pred) =
+  let h0 = get() in
+  match l with 
+  | Nil -> ()
+  | Cons h tlref ->
+      let tl = !tlref in 
+      eliminate_inv_contains h0 (TLList TNat) tlref;
+      deep_declassify tl;
+      let h1 = get () in
+      declassify_low' tlref;
+      let h2 = get () in
+      lemma_declassify_preserves_inv (TLList TNat) tlref h1 h2;
+      ()
+
+let test_declassify (l: linkedList int) : IST unit 
+  (ensures fun h -> satisfy l h contains_pred) 
+  (requires fun _ _ _ -> True) =
+  deep_declassify l;
+  ()
+
+val progr_linked_list_unchanged: 
+  ll: (linkedList int) -> 
+  ctx:(elab_typ (TArr (TLList TNat) TUnit)) ->
+  IST unit 
+    (requires (fun h0 -> satisfy ll h0 contains_pred))
+    (ensures (fun h0 _ h1 -> True))
+  
+[@expect_failure]
+let progr_linked_list_unchanged ll ctx =
+  ctx ll (* call should fail because it does not know that ll is low *)
+
+let progr_linked_list_unchanged ll ctx =
+  deep_declassify ll;
+  ctx ll
+
+// #push-options "--split_queries always"
 // let rec deep_declassify (l: linkedList int) : ST unit 
 //   (requires fun h -> satisfy l h contains_pred /\ inv_contains_points_to_contains h)
 //   (ensures fun h0 x h1 ->
@@ -224,84 +287,88 @@ let cycle_length3 () : ST (linkedList nat) (requires fun _ -> True) (ensures fun
 //     modifies Set.empty h0 h1 /\
 //     (* TODO: modifies_classification (footprint l) h0 h1 *)
 //     satisfy l h1 is_low_pred /\
-//     (forall (a:Type) (c:witnessable a) (r:ref a). 
-//     (~(satisfy r h0 is_low_pred) /\ satisfy r h1 is_low_pred) ==> c.satisfy (sel h1 r) h1 is_low_pred)
+//     (forall (t:typ) (r:ref (elab_typ t)). 
+//       (~((elab_typ_tgt (TRef t)).satisfy r h0 is_low_pred) /\ 
+//        (elab_typ_tgt (TRef t)).satisfy r h1 is_low_pred) ==> 
+//          (elab_typ_tgt t).satisfy (sel h1 r) h1 is_low_pred)
 //     ) =
 //   let h0 = get() in
 //   match l with 
 //   | Nil -> ()
-//   | Cons (h, tlref) ->
+//   | Cons h tlref ->
 //       let tl = !tlref in 
 //       declassify_low' tlref;
-//       eliminate forall (a:Type) (c:witnessable a) (r:ref a). satisfy r h0 contains_pred ==>
-//         c.satisfy (sel h0 r) h0 contains_pred with (linkedList int) (solve) tlref;
+//       eliminate_inv_contains h0 (TLList TNat) tlref;
 //       let h1 = get () in
 //       deep_declassify tl;
 //       let h2 = get () in
-//       introduce forall (a:Type) (c:witnessable a) (r:ref a). 
-//                (~(satisfy r h0 is_low_pred) /\ satisfy r h2 is_low_pred) ==> 
-//                 c.satisfy (sel h2 r) h2 is_low_pred
+//       introduce forall (t:typ) (r:ref (elab_typ t)). 
+//         (~((elab_typ_tgt (TRef t)).satisfy r h0 is_low_pred) /\ 
+//           (elab_typ_tgt (TRef t)).satisfy r h2 is_low_pred) ==> 
+//             (elab_typ_tgt t).satisfy (sel h2 r) h2 is_low_pred
 //       with begin
-//         introduce (~(satisfy r h0 is_low_pred) /\ satisfy r h2 is_low_pred) ==> 
-//                 c.satisfy (sel h2 r) h2 is_low_pred
+//         let wr = elab_typ_tgt t in
+//         introduce (~(satisfy r h0 is_low_pred) /\ satisfy r h2 is_low_pred) 
+//           ==> wr.satisfy (sel h2 r) h2 is_low_pred
 //         with _. begin
-//           introduce ~(satisfy r h1 is_low_pred) ==> c.satisfy (sel h2 r) h2 is_low_pred with _. ();
-//           introduce satisfy r h1 is_low_pred ==> c.satisfy (sel h2 r) h2 is_low_pred with _. begin
+//           introduce ~(satisfy r h1 is_low_pred) ==> wr.satisfy (sel h2 r) h2 is_low_pred with _. ();
+//           introduce satisfy r h1 is_low_pred ==> wr.satisfy (sel h2 r) h2 is_low_pred with _. begin
 //             assert (addr_of r = addr_of tlref);
-//             assume (is_mm r = is_mm tlref);
 //             lemma_sel_same_addr' h2 r tlref;
 //             // assert (shallowly_low (sel h2 tlref) h2);
 //             // assert (sel h2 tlref == sel h2 r);
-//             let c : witnessable (linkedList int) = c in
-//             assert ((target_lang_linkedList int).satisfy (sel h2 tlref) h2 is_low_pred);
-//             assume ((forall (a:Type) (c:witnessable a) (c':witnessable a) (v:a) . 
-//               c.satisfy v h2 is_low_pred ==> c'.satisfy v h2 is_low_pred));
-//             assert (c.satisfy (sel h2 tlref) h2 is_low_pred);
+//             assert ((witnessable_llist int).satisfy (sel h2 tlref) h2 is_low_pred);
+//             assert (wr.satisfy (sel h2 tlref) h2 is_low_pred);
 //             ()
 //           end
 //         end 
 //       end;
 //       ()
+// #pop-options
+
 
 // (* Tests *)
 
 // // TODO: Review this
 // let test_declassify (l: linkedList int) : IST unit 
-//   (ensures fun h -> shallowly_contained l h) 
+//   (ensures fun h -> satisfy l h contains_pred) 
 //   (requires fun _ _ _ -> True) =
 //   let h0 = get() in
 //   deep_declassify l;
 //   let h1 = get() in
-//   // assume ((forall (a:Type) (c:target_lang a) (c':target_lang a) (v:a) . 
-//   //   (target_lang_ref a #c).shallowly_low v h1 ==> c'.shallowly_low v h1));
 
-//   assert (modifies Set.empty h0 h1);
-//   assert (shallowly_contained l h0);
-//   assert (shallowly_contained l h1);
-//   assert (inv_contains_points_to_contains h1);
-
-//   assert (shallowly_low l h1);
-//   assert (inv_low_points_to_low h0); // by IST
-
-//   introduce forall (a:Type) (c:target_lang a) (r:ref a).
-//     shallowly_low r h1 ==> c.shallowly_low (sel h1 r) h1
+//   introduce forall (t:typ) inv.
+//     let tt = _elab_typ t inv in
+//     forall (r:ref (dfst tt)).
+//       (witnessable_ref (dfst tt) #(dsnd tt)).satisfy r h1 is_low_pred ==> 
+//         (dsnd tt).satisfy (sel h1 r) h1 is_low_pred
 //   with begin
-//     introduce shallowly_low r h1 ==> c.shallowly_low (sel h1 r) h1 with _. begin
-//       introduce shallowly_low r h0 ==> c.shallowly_low (sel h1 r) h1 with _. begin
-//         assert (h0 `contains` r);
-//         assert (modifies_none h0 h1);
-//         assert (sel h1 r == sel h0 r);
-//         assert (shallowly_low r h0 ==> c.shallowly_low (sel h0 r) h0);
-//         lemma (sel h1 r) h0 h1;
-//         // assume (shallowly_low (sel h1 r) h0 ==> shallowly_low (sel h1 r) h1);
-//         ()
-//       end;
-//       introduce ~(shallowly_low r h0) ==> c.shallowly_low (sel h1 r) h1 with _. begin
-//         assert
-//           ((~(shallowly_low r h0) /\ shallowly_low r h1) ==> c.shallowly_low (sel h1 r) h1);
-//         assert (~(shallowly_low r h0));
-//         assert (shallowly_low r h1);
-//         ()
+//     let tt = _elab_typ t inv in
+//     let refw = witnessable_ref (dfst tt) #(dsnd tt) in
+//     introduce forall (r:ref (dfst tt)).
+//       refw.satisfy r h1 is_low_pred ==> 
+//         (dsnd tt).satisfy (sel h1 r) h1 is_low_pred
+//     with begin
+//       let wr = dsnd tt in
+//       introduce satisfy r h1 is_low_pred ==> wr.satisfy (sel h1 r) h1 is_low_pred with _. begin
+//         introduce satisfy r h0 is_low_pred ==> wr.satisfy (sel h1 r) h1 is_low_pred with _. begin
+//           assert (h0 `contains` r);
+//           assert (modifies_none h0 h1);
+//           assert (sel h1 r == sel h0 r);
+//           assert (satisfy r h0 is_low_pred ==> wr.satisfy (sel h0 r) h0 is_low_pred);
+
+//           wr.satisfy_monotonic (sel h1 r) is_low_pred h0 h1;
+//           // assume (shallowly_low (sel h1 r) h0 ==> shallowly_low (sel h1 r) h1);
+//           ()
+//         end;
+//         introduce ~(satisfy r h0 is_low_pred) ==> wr.satisfy (sel h1 r) h1 is_low_pred with _. begin
+//           assert
+//             ((~(satisfy r h0 is_low_pred) /\ satisfy r h1 is_low_pred) ==> 
+//               wr.satisfy (sel h1 r) h1 is_low_pred);
+//           assert (~(satisfy r h0 is_low_pred));
+//           assert (satisfy r h1 is_low_pred);
+//           ()
+//         end
 //       end
 //     end
 //   end;
